NLustreToSyBloc/Correctness.v
@@ -1,0 +1,397 @@
+Require Import Coq.FSets.FMapPositive.
+Require Import PArith.
+Require Import Velus.Common.
+Require Import Velus.Operators.
+Require Import Velus.Clocks.
+Require Import Velus.NLustre.NLSyntax.
+Require Import Velus.NLustre.Memories.
+Require Import Velus.SyBloc.SBSyntax.
+Require Import Velus.NLustre.Ordered.
+Require Import Velus.NLustre.Stream.
+Require Import Velus.NLustre.NLSemantics.
+Require Import Velus.SyBloc.SBSemantics.
+Require Import Velus.NLustreToSyBloc.Translation.
+Require Import Velus.RMemory.
+
+Require Import List.
+Import List.ListNotations.
+Require Import Coq.Sorting.Permutation.
+Require Import Morphisms.
+
+Open Scope list.
+Open Scope nat.
+
+Module Type CORRECTNESS
+       (Import Ids   : IDS)
+       (Import Op    : OPERATORS)
+       (Import OpAux : OPERATORS_AUX Op)
+       (Import Clks  : CLOCKS      Ids)
+       (Import SynNL : NLSYNTAX    Ids Op       Clks)
+       (SynSB        : SBSYNTAX    Ids Op       Clks)
+       (Import Str   : STREAM          Op OpAux)
+       (Import Ord   : ORDERED     Ids Op       Clks SynNL)
+       (Import SemNL : NLSEMANTICS Ids Op OpAux Clks SynNL       Str Ord)
+       (SemSB        : SBSEMANTICS Ids Op OpAux Clks       SynSB Str)
+       (Import Mem   : MEMORIES    Ids Op       Clks SynNL)
+       (Import Trans : TRANSLATION Ids Op       Clks SynNL SynSB Mem).
+
+  (* Fixpoint memvar_lexp (x: ident) (e: SynSB.lexp) := *)
+  (*   match e with *)
+  (*   | SynSB.Emem y _ => x = y *)
+  (*   | SynSB.Ewhen e _ _ => memvar_lexp x e *)
+  (*   | SynSB.Eunop _ e _ => memvar_lexp x e *)
+  (*   | SynSB.Ebinop _ e1 e2 _ => memvar_lexp x e1 \/ memvar_lexp x e2 *)
+  (*   | _ => False *)
+  (*   end. *)
+
+  (* Fixpoint memvar_cexp (x: ident) (ce: SynSB.cexp) := *)
+  (*   match ce with *)
+  (*   | SynSB.Emerge _ e1 e2 => memvar_cexp x e1 \/ memvar_cexp x e2 *)
+  (*   | SynSB.Eite e t f => memvar_lexp x e \/ memvar_cexp x t \/ memvar_cexp x f *)
+  (*   | SynSB.Eexp e => memvar_lexp x e *)
+  (*   end. *)
+
+  Definition memory_spec (m: SemSB.memory) (memids: PS.t) (R: env) :=
+    forall x v,
+      PM.find x R = Some v ->
+      PS.mem x memids = true ->
+      SemSB.get_reg x m = Some v.
+
+  Definition memories_spec (M: SemSB.memories) (memids: PS.t) (H: history) :=
+    forall n, memory_spec (SemSB.restr_mem M n) memids (SemSB.restr_hist H n).
+
+  Section Global.
+
+    Variable G: SynNL.global.
+    Let P := translate G.
+
+    Section SemInstant.
+
+      Variable base: bool.
+      Variable R: env.
+
+      Lemma var_instant_correctness:
+        forall x v,
+          sem_var_instant R x v ->
+          SemSB.sem_var_instant R x v.
+      Proof.
+        induction 1; constructor; auto.
+      Qed.
+      Hint Resolve var_instant_correctness.
+
+      Lemma clock_instant_correctness:
+        forall ck b,
+          sem_clock_instant base R ck b ->
+          SemSB.sem_clock_instant base R ck b.
+      Proof.
+        induction 1; eauto using SemSB.sem_clock_instant.
+      Qed.
+
+      Variable m: SemSB.memory.
+      Variable memids: PS.t.
+      (* Variable mems: list (ident * const). *)
+      (* Let memids := ps_from_list (map fst mems). *)
+
+      Lemma typeof_correctness:
+        forall e,
+          SynSB.typeof (translate_lexp memids e) = typeof e.
+      Proof.
+        induction e; intros; simpl; auto.
+        destruct (PS.mem i memids); auto.
+      Qed.
+      (* Hint Resolve typeof_correctness. *)
+
+      Hypothesis Spec: memory_spec m memids R.
+
+      Lemma lexp_instant_correctness:
+        forall e v,
+          sem_lexp_instant base R e v ->
+          SemSB.sem_lexp_instant base R m (translate_lexp memids e) v.
+      Proof.
+        induction 1; simpl; eauto using SemSB.sem_lexp_instant.
+        - destruct (PS.mem x memids) eqn: E.
+          + do 2 constructor.
+            unfold SemSB.get_reg.
+            match goal with H: sem_var_instant R x v |- _ =>
+                            inversion_clear H as [?? Find] end.
+            apply Spec; auto.
+          + eauto using SemSB.sem_lexp_instant.
+        - econstructor; eauto.
+          now rewrite typeof_correctness.
+        - econstructor; eauto.
+          now rewrite 2 typeof_correctness.
+      Qed.
+      Hint Resolve lexp_instant_correctness.
+
+      Lemma lexps_instant_correctness:
+        forall es vs,
+          sem_lexps_instant base R es vs ->
+          SemSB.sem_lexps_instant base R m (map (translate_lexp memids) es) vs.
+      Proof.
+        induction 1; constructor; auto.
+      Qed.
+
+      Lemma cexp_instant_correctness:
+        forall ce v,
+          sem_cexp_instant base R ce v ->
+          SemSB.sem_cexp_instant base R m (translate_cexp memids ce) v.
+      Proof.
+        induction 1; simpl; eauto using SemSB.sem_cexp_instant.
+      Qed.
+
+      (* Lemma sem_lexp_instant_madd_mem: *)
+      (*   forall x mv e v, *)
+      (*     SemSB.sem_lexp_instant base R m e v -> *)
+      (*     ~ memvar_lexp x e -> *)
+      (*     SemSB.sem_lexp_instant base R (madd_mem x mv m) e v. *)
+      (* Proof. *)
+      (*   induction 1; simpl; intros Nmv; eauto using SemSB.sem_lexp_instant. *)
+      (*   - do 2 constructor. *)
+      (*     match goal with H: SemSB.sem_mem_var_instant _ _ _ |- _ => inv H end. *)
+      (*     unfold SemSB.get_mem in *. *)
+      (*     rewrite mfind_mem_gso; auto. *)
+      (*   - econstructor; eauto. *)
+      (*   - econstructor; eauto. *)
+      (* Qed. *)
+      (* Hint Resolve sem_lexp_instant_madd_mem. *)
+
+      (* Lemma sem_cexp_instant_madd_mem: *)
+      (*   forall x mv ce v, *)
+      (*     SemSB.sem_cexp_instant base R m ce v -> *)
+      (*     ~ memvar_cexp x ce -> *)
+      (*     SemSB.sem_cexp_instant base R (madd_mem x mv m) ce v. *)
+      (* Proof. *)
+      (*   induction 1; simpl; intros Nmv; eauto using SemSB.sem_cexp_instant. *)
+      (*   - econstructor; eauto. *)
+      (*   - econstructor 2; eauto. *)
+      (*   - econstructor; eauto. *)
+      (*   - econstructor; eauto. *)
+      (*     + apply IHsem_cexp_instant1; auto. *)
+      (*     + apply IHsem_cexp_instant2; auto. *)
+      (*   - econstructor; eauto. *)
+      (*     + apply IHsem_cexp_instant1; auto. *)
+      (*     + apply IHsem_cexp_instant2; auto. *)
+      (* Qed. *)
+
+      (* Lemma sem_lexps_instant_madd_mem: *)
+      (*   forall x mv es vs, *)
+      (*     SemSB.sem_lexps_instant base R m es vs -> *)
+      (*     Forall (fun e => ~ memvar_lexp x e) es -> *)
+      (*     SemSB.sem_lexps_instant base R (madd_mem x mv m) es vs. *)
+      (* Proof. *)
+      (*   induction 1; simpl; intros Nmv; inv Nmv. *)
+      (*   - constructor. *)
+      (*   - constructor; auto. *)
+      (*     apply IHForall2; auto. *)
+      (* Qed. *)
+
+    End SemInstant.
+    Hint Resolve var_instant_correctness clock_instant_correctness
+         lexp_instant_correctness lexps_instant_correctness
+         cexp_instant_correctness.
+         (* sem_cexp_instant_madd_mem sem_lexps_instant_madd_mem. *)
+
+    Lemma pm_map_add:
+      forall {A B} (m: PM.t A) (f: A -> B) x v,
+        PM.map f (PM.add x v m) = PM.add x (f v) (PM.map f m).
+    Proof.
+    Admitted.
+
+    Lemma restr_mem_madd_mem:
+      forall x mvs M n,
+        SemSB.restr_mem (madd_mem x mvs M) n =
+        madd_mem x (SemSB.restr_mvalues n mvs) (SemSB.restr_mem M n).
+    Proof.
+      intros.
+      unfold SemSB.restr_mem, madd_mem; simpl.
+      f_equal.
+      - now rewrite pm_map_add, mm_values_map.
+      - now rewrite mm_instances_map.
+    Qed.
+
+    Section Sem.
+
+      Variable bk: stream bool.
+      Variable H: history.
+
+      Lemma var_correctness:
+        forall x xs,
+          sem_var bk H x xs ->
+          SemSB.sem_var H x xs.
+      Proof.
+        intros ** Sem n; specialize (Sem n); auto.
+      Qed.
+      Hint Resolve var_correctness.
+
+      Lemma vars_correctness:
+        forall xs xss,
+          sem_vars bk H xs xss ->
+          SemSB.sem_vars H xs xss.
+      Proof.
+        intros ** Sem n; specialize (Sem n);
+          induction Sem; constructor; auto.
+      Qed.
+
+      Variable M: SemSB.memories.
+      Variable memids: PS.t.
+      Hypothesis Spec: memories_spec M memids H.
+      (* Variable mems: list (ident * const). *)
+      (* Let memids := ps_from_list (map fst mems). *)
+
+      Lemma laexp_correctness:
+        forall ck e xs,
+          sem_laexp bk H ck e xs ->
+          SemSB.sem_laexp bk H M ck (translate_lexp memids e) xs.
+      Proof.
+        intros ** Sem n; specialize (Sem n); simpl in Sem.
+        induction Sem; constructor; auto.
+      Qed.
+
+      Lemma caexp_correctness:
+        forall ck ce xs,
+          sem_caexp bk H ck ce xs ->
+          SemSB.sem_caexp bk H M ck (translate_cexp memids ce) xs.
+      Proof.
+        intros ** Sem n; specialize (Sem n); simpl in Sem.
+        induction Sem; constructor; auto.
+      Qed.
+
+      Lemma laexps_correctness:
+        forall ck es vs,
+          sem_laexps bk H ck es vs ->
+          SemSB.sem_laexps bk H M ck (map (translate_lexp memids) es) vs.
+      Proof.
+        intros ** Sem n; specialize (Sem n); inv Sem.
+        - econstructor 1; eauto.
+        - constructor; auto.
+          now rewrite all_absent_map.
+      Qed.
+
+      Lemma sem_caexp_laexp:
+        forall ck e xs,
+          SemSB.sem_caexp bk H M ck (SynSB.Eexp e) xs
+          <-> SemSB.sem_laexp bk H M ck e xs.
+      Proof.
+        split; intros ** Sem n; specialize (Sem n).
+        - inv Sem; match goal with H: SemSB.sem_cexp_instant _ _ _ _ _ |- _ => inv H end;
+            constructor; auto.
+        - induction Sem; repeat constructor; auto.
+      Qed.
+
+      (* Lemma sem_caexp_madd_mem: *)
+      (*   forall x mvs ck ce xs, *)
+      (*     SemSB.sem_caexp bk H M ck ce xs -> *)
+      (*     ~ memvar_cexp x ce -> *)
+      (*     SemSB.sem_caexp bk H (madd_mem x mvs M) ck ce xs. *)
+      (* Proof. *)
+      (*   intros ** Sem ? n; specialize (Sem n); inv Sem; *)
+      (*     econstructor; eauto; *)
+      (*       rewrite restr_mem_madd_mem; auto. *)
+      (* Qed. *)
+
+      (* Lemma sem_laexps_madd_mem: *)
+      (*   forall x mvs ck es xss, *)
+      (*     SemSB.sem_laexps bk H M ck es xss -> *)
+      (*     Forall (fun e => ~ memvar_lexp x e) es -> *)
+      (*     SemSB.sem_laexps bk H (madd_mem x mvs M) ck es xss. *)
+      (* Proof. *)
+      (*   intros ** Sem ? n; specialize (Sem n); inv Sem. *)
+      (*   - econstructor; eauto. *)
+      (*     rewrite restr_mem_madd_mem; auto. *)
+      (*   - econstructor 2; eauto. *)
+      (*     rewrite restr_mem_madd_mem; auto. *)
+      (*   - constructor 3. *)
+      (* Qed. *)
+
+      (* Lemma sem_equation_madd_mem: *)
+      (*   forall x mvs mems k eqs, *)
+      (*     (* ~Is_defined_in_eqs x eqs -> *) *)
+      (*     Forall (SemSB.sem_equation P k bk H M mems) eqs -> *)
+      (*     Forall (SemSB.sem_equation P k bk H (madd_mem x mvs M) mems) eqs. *)
+      (* Proof. *)
+      (*   intros ** (* Hnd *) Hsem. *)
+      (*   induction eqs as [|eq eqs IH]; [now constructor|]. *)
+      (*   (* apply not_Is_defined_in_cons in Hnd. *) *)
+      (*   (* destruct Hnd as [Hnd Hnds]. *) *)
+      (*   apply Forall_cons2 in Hsem as [Hsem Hsems]. *)
+      (*   constructor; auto. *)
+      (*   destruct Hsem; eauto using SemSB.sem_equation. *)
+      (*   - econstructor; eauto. *)
+      (*     apply sem_caexp_madd_mem; auto. *)
+      (*     admit. *)
+      (*   - admit. *)
+      (*   - econstructor; eauto. *)
+      (*     apply sem_laexps_madd_mem; auto. *)
+      (*     admit. *)
+      (* Admitted. *)
+
+    End Sem.
+    Hint Resolve var_correctness vars_correctness
+         laexp_correctness caexp_correctness laexps_correctness.
+
+
+    Theorem correctness:
+      forall f xss oss,
+        sem_node G f xss oss ->
+        exists M, SemSB.sem_block P f M xss oss.
+    Proof.
+      induction 1 as [| | | |???? IHNode|] using sem_node_mult with
+          (P_equation := fun b H e =>
+                           (* sem_equation G b H e -> *)
+                           exists M mems,
+                             memories_spec M (ps_from_list (map (@fst ident const) mems)) H ->
+                             Forall (SemSB.sem_equation P b H M)
+                                    (translate_eqn (ps_from_list (map fst mems)) e))
+          (P_reset := fun f r xss oss =>
+                        (* sem_reset G f r xss oss -> *)
+                        exists M, SemSB.sem_block P f M xss oss
+                             /\ SemSB.reset_regs r M
+          );
+        eauto.
+      - repeat (econstructor; eauto).
+
+      -
+        (* intro Sem; clear Sem. *)
+        destruct IHsem_node as (M & Sem).
+        match goal with
+          H: sem_node _ _ _ _ |- _ =>
+          inversion_clear H as [??????? Find]
+        end.
+        apply find_node_translate in Find as (bl & ? & Find & E).
+        subst.
+        simpl.
+        exists (madd_obj (hd default x) M (@empty_memory SemSB.mvalues)).
+        repeat (econstructor; eauto);
+          apply mfind_inst_gss.
+
+      -
+        (* intro Sem; clear Sem. *)
+        destruct IHsem_node as (M & Block & Reset); auto.
+        match goal with H: sem_reset _ _ _ _ _ |- _ => inversion_clear H as [???? Sem] end.
+        simpl.
+        exists (madd_obj (hd default x) M (@empty_memory SemSB.mvalues)).
+        econstructor.
+        pose proof (Sem 0) as Sem0; inv Sem0.
+        edestruct find_node_translate as (bl & P' & ? & ?); eauto.
+        subst.
+        repeat (econstructor; eauto);
+          apply mfind_inst_gss.
+
+      -
+        (* intro Sem; clear Sem; simpl. *)
+        exists (madd_mem x {| SemSB.content := xs; SemSB.reset := fun _ => false; SemSB.init := c0 |} (@empty_memory SemSB.mvalues)).
+        exists [(x, c0)].
+        econstructor; eauto.
+        econstructor; eauto.
+        + apply sem_caexp_laexp; eauto.
+        + econstructor.
+          * apply mfind_mem_gss.
+          * simpl; intro n.
+            subst. unfold fby. simpl.
+            admit.
+
+      - admit.
+
+      - admit.
+
+    Qed.
