SyBloc/SBSyntax.v
@@ -1,0 +1,202 @@
+Require Import Velus.Common.
+Require Import Velus.Operators.
+Require Import Velus.Clocks.
+(* Require Import PArith. *)
+(* Require Import Coq.Sorting.Permutation. *)
+
+Require Import List.
+Import List.ListNotations.
+Open Scope list_scope.
+
+
+Module Type SBSYNTAX
+       (Import Ids  : IDS)
+       (Import Op   : OPERATORS)
+       (Import Clks : CLOCKS Ids).
+
+  (** ** Expressions *)
+
+  Inductive lexp :=
+  | Econst : const -> lexp
+  | Evar   : ident -> type -> lexp
+  | Ereg   : ident -> type -> lexp
+  | Ewhen  : lexp -> ident -> bool -> lexp
+  | Eunop  : unop -> lexp -> type -> lexp
+  | Ebinop : binop -> lexp -> lexp -> type -> lexp.
+
+  (** ** Control expressions *)
+
+  Inductive cexp :=
+  | Emerge : ident -> cexp -> cexp -> cexp
+  | Eite   : lexp -> cexp -> cexp -> cexp
+  | Eexp   : lexp -> cexp.
+
+  (** ** Equations *)
+
+  Inductive equation :=
+  | EqDef : ident -> clock -> cexp -> equation
+  | EqReg : ident -> clock -> cexp -> equation
+  | EqReset : clock -> ident -> ident -> ident -> equation (* reinit block instance on r *)
+  | EqCall: idents -> clock -> ident -> ident -> list lexp -> equation.
+  (* y1, ..., yn = block instance (e1, ..., em) *)
+
+  Record block :=
+    Block {
+        b_name  : ident;
+        b_in    : list (ident * type);
+        b_vars  : list (ident * type);
+        b_regs  : list (ident * const);
+        b_blocks: list (ident * ident);
+        b_out   : list (ident * type);
+        b_eqs   : list equation
+      }.
+
+  Definition program := list block.
+
+  Fixpoint typeof (le: lexp): type :=
+    match le with
+    | Econst c => type_const c
+    | Evar _ ty
+    | Ereg _ ty
+    | Eunop _ _ ty
+    | Ebinop _ _ _ ty => ty
+    | Ewhen e _ _ => typeof e
+    end.
+
+  (* Fixpoint find_mode (m: ident) (ms: list mode): option mode := *)
+  (*   match ms with *)
+  (*   | [] => None *)
+  (*   | mo :: ms => *)
+  (*     if ident_eqb mo.(m_name) m *)
+  (*     then Some mo else find_mode m ms *)
+  (*   end. *)
+
+  (* Remark find_mode_In: *)
+  (*   forall m ms mo, *)
+  (*     find_mode m ms = Some mo -> *)
+  (*     In mo ms. *)
+  (* Proof. *)
+  (*   intros ** Hfind. *)
+  (*   induction ms; inversion Hfind as [H]. *)
+  (*   destruct (ident_eqb (m_name a) m) eqn: E. *)
+  (*   - inversion H; subst. *)
+  (*     apply in_eq. *)
+  (*   - auto using in_cons. *)
+  (* Qed. *)
+
+  (* Remark find_mode_name: *)
+  (*   forall m ms mo, *)
+  (*     find_mode m ms = Some mo -> *)
+  (*     mo.(m_name) = m. *)
+  (* Proof. *)
+  (*   intros ** Hfind. *)
+  (*   induction ms; inversion Hfind as [H]. *)
+  (*   destruct (ident_eqb (m_name a) m) eqn: E. *)
+  (*   - inversion H; subst. *)
+  (*     now apply ident_eqb_eq. *)
+  (*   - now apply IHms. *)
+  (* Qed. *)
+
+  Fixpoint find_block (b: ident) (P: program) : option (block * program) :=
+   match P with
+   | [] => None
+   | bl :: P =>
+     if ident_eqb bl.(b_name) b
+     then Some (bl, P) else find_block b P
+   end.
+
+  (** Properties of block lookups *)
+
+  Lemma find_block_none:
+    forall b bl P,
+      find_block b (bl :: P) = None
+      <-> (bl.(b_name) <> b /\ find_block b P = None).
+  Proof.
+    intros.
+    simpl; destruct (ident_eqb (b_name bl) b) eqn: E.
+    - split; intro HH; try discriminate.
+      destruct HH.
+      apply ident_eqb_eq in E; contradiction.
+    - apply ident_eqb_neq in E; split; intro HH; tauto.
+  Qed.
+
+  Remark find_block_app:
+    forall b P bl P',
+      find_block b P = Some (bl, P') ->
+      exists P'',
+        P = P'' ++ bl :: P'
+        /\ find_block b P'' = None.
+  Proof.
+    intros ** Hfind.
+    induction P; inversion Hfind as [H].
+    destruct (ident_eqb (b_name a) b) eqn: E.
+    - inversion H; subst.
+      exists nil; auto.
+    - specialize (IHP H).
+      destruct IHP as (P'' & HP'' & Hnone).
+      rewrite HP''.
+      exists (a :: P''); split; auto.
+      simpl; rewrite E; auto.
+  Qed.
+
+  Remark find_block_name:
+    forall b P bl P',
+      find_block b P = Some (bl, P') ->
+      bl.(b_name) = b.
+  Proof.
+    intros ** Hfind.
+    induction P; inversion Hfind as [H].
+    destruct (ident_eqb (b_name a) b) eqn: E.
+    - inversion H; subst.
+      now apply ident_eqb_eq.
+    - now apply IHP.
+  Qed.
+
+  Remark find_block_In:
+    forall b P bl P',
+      find_block b P = Some (bl, P') ->
+      In bl P.
+  Proof.
+    intros ** Hfind.
+    induction P; inversion Hfind as [H].
+    destruct (ident_eqb (b_name a) b) eqn: E.
+    - inversion H; subst.
+      apply in_eq.
+    - apply in_cons; auto.
+  Qed.
+
+  Lemma find_block_app':
+    forall b P P',
+      find_block b (P ++ P') =
+      match find_block b P with
+      | None => find_block b P'
+      | Some (bl, P'') => Some (bl, P'' ++ P')
+      end.
+  Proof.
+    induction P as [|bl P]; simpl; auto.
+    intro; destruct (ident_eqb bl.(b_name) b); auto.
+  Qed.
+
+  Lemma not_In_find_block:
+    forall b P,
+      ~In b (map b_name P) ->
+      find_block b P = None.
+  Proof.
+    induction P as [|bl]; auto.
+    simpl; intro Hnin.
+    apply Decidable.not_or in Hnin.
+    destruct Hnin as (Hnin1 & Hnin2).
+    rewrite (IHP Hnin2).
+    apply ident_eqb_neq in Hnin1.
+    now rewrite Hnin1.
+  Qed.
+
+End SBSYNTAX.
+
+Module SBSyntaxFun
+       (Ids  : IDS)
+       (Op   : OPERATORS)
+       (Clks : CLOCKS Ids)
+       <: SBSYNTAX Ids Op Clks.
+  Include SBSYNTAX Ids Op Clks.
+End SBSyntaxFun.
